@prefix : <http://example.org/stilton#> .
@prefix owl: <http://www.w3.org/2002/07/owl#> .
@prefix rdf: <http://www.w3.org/1999/02/22-rdf-syntax-ns#> .
@prefix xml: <http://www.w3.org/XML/1998/namespace> .
@prefix xsd: <http://www.w3.org/2001/XMLSchema#> .
@prefix rdfs: <http://www.w3.org/2000/01/rdf-schema#> .
@prefix schema: <https://schema.org/> .
@base <http://example.org/stilton#> .

[ rdf:type owl:Ontology
 ] .

#################################################################
#    Object Properties
#################################################################

###  http://example.org/stilton#hasAunt
:hasAunt rdf:type owl:ObjectProperty ;
         rdfs:domain :Character ,
                     schema:Person ;
         rdfs:range :Character ,
                    schema:Person ;
         rdfs:comment "Relates a character to their aunt, who is the sister of one of the character's parents."@en .


###  http://example.org/stilton#hasCousin
:hasCousin rdf:type owl:ObjectProperty ;
           rdfs:subPropertyOf owl:topObjectProperty ;
           rdf:type owl:SymmetricProperty ;
           rdfs:domain :Character ,
                       schema:Person ;
           rdfs:range :Character ,
                      schema:Person ;
           rdfs:comment "Represents a reciprocal family relationship between characters who are children of siblings (i.e., first cousins). This property is symmetric, meaning if Character A is a cousin of Character B, then Character B is also a cousin of Character A."@en .


###  http://example.org/stilton#hasFriend
:hasFriend rdf:type owl:ObjectProperty ,
                    owl:SymmetricProperty ;
           rdfs:domain :Character ,
                       schema:Person ;
           rdfs:range :Character ,
                      schema:Person ;
           rdfs:comment "Denotes a bidirectional friendship between two characters."@en .


###  http://example.org/stilton#hasGrandParent
:hasGrandParent rdf:type owl:ObjectProperty ;
                rdfs:subPropertyOf owl:topObjectProperty ;
                rdfs:domain :Character ,
                            schema:Person ;
                rdfs:range :Character ,
                           schema:Person ;
                rdfs:comment "Relates a character to their grandparent, who is the parent of one of their parents."@en .


###  http://example.org/stilton#hasNephew
:hasNephew rdf:type owl:ObjectProperty ;
           rdfs:domain :Character ,
                       schema:Person ;
           rdfs:range :Character ,
                      schema:Person ;
           rdfs:comment "Relates a character to a nephew, defined as the son of their sibling."@en .


###  http://example.org/stilton#hasNiece
:hasNiece rdf:type owl:ObjectProperty ;
          rdfs:domain :Character ,
                      schema:Person ;
          rdfs:range :Character ,
                     schema:Person ;
          rdfs:comment "Relates a character to a niece, defined as the daughter of their sibling."@en .


###  http://example.org/stilton#hasSibling
:hasSibling rdf:type owl:ObjectProperty ,
                     owl:SymmetricProperty ,
                     owl:TransitiveProperty ;
            rdfs:domain :Character ,
                        schema:Person ;
            rdfs:range :Character ,
                       schema:Person ;
            rdfs:comment "Denotes a sibling relationship between characters who share the same parents. This property is both symmetric and transitive."@en .


###  http://example.org/stilton#hasUncle
:hasUncle rdf:type owl:ObjectProperty ;
          rdfs:subPropertyOf owl:topObjectProperty ;
          rdfs:domain :Character ,
                      schema:Person ;
          rdfs:range :Character ,
                     schema:Person ;
          rdfs:comment "Relates a character to their uncle, who is the brother of one of the characterâ€™s parents."@en .


###  http://example.org/stilton#memberOfGroup
:memberOfGroup rdf:type owl:ObjectProperty ;
               rdfs:domain :Character ,
                           schema:Person ;
               rdfs:range :Group ;
               rdfs:comment "Relates a character to a group they belong to, such as a family unit, team, or organization."@en .


###  https://schema.org/employee
schema:employee rdf:type owl:ObjectProperty ;
                rdfs:domain schema:Organization ;
                rdfs:range :Character ,
                           schema:Person .


###  https://schema.org/homeLocation
schema:homeLocation rdf:type owl:ObjectProperty ;
                    rdfs:range schema:Place .


###  https://schema.org/worksFor
schema:worksFor rdf:type owl:ObjectProperty ;
                rdfs:domain :Character ,
                            schema:Person ;
                rdfs:range schema:Organization .


#################################################################
#    Data properties
#################################################################

###  http://www.w3.org/2004/02/skos/core#altLabel
<http://www.w3.org/2004/02/skos/core#altLabel> rdf:type owl:DatatypeProperty .


###  https://schema.org/jobTitle
schema:jobTitle rdf:type owl:DatatypeProperty ;
                rdfs:range xsd:string .


#################################################################
#    Classes
#################################################################

###  http://example.org/stilton#Character
:Character rdf:type owl:Class ;
           owl:equivalentClass schema:Person ;
           rdfs:comment "A fictional character from the Geronimo Stilton universe. Characters may have relationships such as family ties or friendships."@en .


###  http://example.org/stilton#Group
:Group rdf:type owl:Class ;
       rdfs:comment "A collection of characters who are part of an organized team, band, or family unit."@en ;
       rdfs:label "Group"@en .


###  https://schema.org/Organization
schema:Organization rdf:type owl:Class .


###  https://schema.org/Person
schema:Person rdf:type owl:Class .


###  https://schema.org/Place
schema:Place rdf:type owl:Class .


#################################################################
#    Individuals
#################################################################

###  http://example.org/stilton#Blossom
:Blossom rdf:type owl:NamedIndividual ,
                  :Character ;
         rdfs:label "Blossom"@en .


###  http://example.org/stilton#Cackle
:Cackle rdf:type owl:NamedIndividual ,
                 :Character ;
        rdfs:label "Cackle"@en .


###  http://example.org/stilton#Clever
:Clever rdf:type owl:NamedIndividual ,
                 :Character ;
        rdfs:label "Clever"@en .


###  http://example.org/stilton#Crowbar
:Crowbar rdf:type owl:NamedIndividual ,
                  :Character ;
         rdfs:label "Crowbar"@en .


###  http://example.org/stilton#George
:George rdf:type owl:NamedIndividual ,
                 :Character ;
        rdfs:label "George"@en .


###  http://example.org/stilton#HerculePoirat
:HerculePoirat rdf:type owl:NamedIndividual ,
                        :Character ;
               rdfs:label "Hercule Poirat"@en .


###  http://example.org/stilton#Lady_of_Dreams
:Lady_of_Dreams rdf:type owl:NamedIndividual ,
                         :Character ;
                rdfs:label "Lady of Dreams"@en .


###  http://example.org/stilton#Mel
:Mel rdf:type owl:NamedIndividual ,
              :Character ;
     rdfs:label "Mel the Magnificent"@en .


###  http://example.org/stilton#PetuniaPrettyPaws
:PetuniaPrettyPaws rdf:type owl:NamedIndividual ,
                            :Character ;
                   rdfs:label "Petunia Pretty Paws"@en .


###  http://example.org/stilton#ProfessorPawsVonVolt
:ProfessorPawsVonVolt rdf:type owl:NamedIndividual ,
                               :Character ;
                      rdfs:label "Professor Paws von Volt"@en .


###  http://example.org/stilton#RodentsGazette
:RodentsGazette rdf:type owl:NamedIndividual ,
                         schema:Organization ;
                schema:employee :geronimoStilton ,
                                :theaStilton ;
                rdfs:label "The Rodents Gazette"@en .


###  http://example.org/stilton#The_Kingdom_of_Fantasy
:The_Kingdom_of_Fantasy rdf:type owl:NamedIndividual ,
                                 schema:Place ;
                        rdfs:label "The Kingdom of Fantasy"@en .


###  http://example.org/stilton#Wither
:Wither rdf:type owl:NamedIndividual ,
                 :Character ;
        rdfs:label "Wither"@en .


###  http://example.org/stilton#benjaminStilton
:benjaminStilton rdf:type owl:NamedIndividual ,
                          :Character ;
                 :hasAunt :theaStilton ;
                 :hasUncle :geronimoStilton ;
                 schema:homeLocation :newMouseCity ;
                 schema:jobTitle "Student" ;
                 rdfs:label "Benjamin Stilton"@en .


###  http://example.org/stilton#geronimoStilton
:geronimoStilton rdf:type owl:NamedIndividual ,
                          :Character ;
                 :hasAunt :sweetfur ;
                 :hasCousin :trapStilton ;
                 :hasFriend :HerculePoirat ,
                            :PetuniaPrettyPaws ,
                            :ProfessorPawsVonVolt ;
                 :hasGrandParent :williamShortpaws ;
                 :hasNephew :benjaminStilton ;
                 :hasSibling :theaStilton ;
                 schema:homeLocation :newMouseCity ;
                 schema:worksFor :RodentsGazette ;
                 <http://www.w3.org/2004/02/skos/core#altLabel> "Gerry Berry" ;
                 schema:jobTitle "Journalist" ;
                 rdfs:label "Geronimo Stilton"@en .


###  http://example.org/stilton#newMouseCity
:newMouseCity rdf:type owl:NamedIndividual ,
                       schema:Place ;
              rdfs:label "New Mouse City" .


###  http://example.org/stilton#sweetfur
:sweetfur rdf:type owl:NamedIndividual ,
                   :Character ;
          :hasNephew :geronimoStilton ,
                     :trapStilton ;
          :hasNiece :theaStilton ;
          rdfs:label "Sweetfur"@en .


###  http://example.org/stilton#theaStilton
:theaStilton rdf:type owl:NamedIndividual ,
                      :Character ;
             :hasAunt :sweetfur ;
             :hasCousin :trapStilton ;
             :hasGrandParent :williamShortpaws ;
             :hasNephew :benjaminStilton ;
             :hasSibling :geronimoStilton ;
             schema:homeLocation :newMouseCity ;
             schema:worksFor :RodentsGazette ;
             schema:jobTitle "Journalist" ,
                             "Nature Photographer" ;
             rdfs:label "Thea Stilton"@en .


###  http://example.org/stilton#trapStilton
:trapStilton rdf:type owl:NamedIndividual ,
                      :Character ;
             :hasAunt :sweetfur ;
             :hasCousin :geronimoStilton ,
                        :theaStilton ;
             :hasGrandParent :williamShortpaws ;
             schema:homeLocation :newMouseCity ;
             schema:jobTitle "Shop owner" ;
             rdfs:label "Trap Stilton"@en .


###  http://example.org/stilton#williamShortpaws
:williamShortpaws rdf:type owl:NamedIndividual ,
                           :Character ;
                  schema:homeLocation :newMouseCity ;
                  rdfs:label "William Shortpaws"@en .


###  Generated by the OWL API (version 4.5.29.2024-05-13T12:11:03Z) https://github.com/owlcs/owlapi
